Total correctness for term equality.

primitives.v
@@ -1,6 +1,7 @@
 From mathcomp Require Import ssreflect.
 From stdpp Require Import gmap.
 From iris.algebra Require Import agree auth gmap.
+From iris.base_logic.lib Require Import invariants.
 From iris.heap_lang Require Import notation proofmode.
 From crypto Require Import term crypto1.
 
@@ -27,24 +28,35 @@ Definition eq_term : val := (rec: "eq" "x" "y" :=
     ("eq" (Snd (Snd "x")) (Snd (Snd "y")))
   else #false)%V.
 
+Definition resN := nroot .@ "res".
+
 Section Proofs.
 
 Context `{!heapG Σ, !resG Σ}.
 
-Lemma wp_eq_term t1 t2 :
-  ⊢ WP (eq_term (val_of_term t1) (val_of_term t2)) {{ v,
-      ⌜v = #(bool_decide (t1 = t2))⌝ }}.
+Implicit Types E : coPset.
+Implicit Types rs : readers.
+
+Definition res_ctx : iProp Σ :=
+  inv resN res_inv.
+
+Global Instance persistent_res_ctx : Persistent res_ctx.
+Proof. apply _. Qed.
+
+Lemma twp_eq_term t1 t2 :
+  ⊢ WP (eq_term (val_of_term t1) (val_of_term t2))
+       [{ v, ⌜v = #(bool_decide (t1 = t2))⌝ }].
 Proof.
-iLöb as "IH" forall (t1 t2).
-case: t1=> [n1|t11 t12|l1|l1 b1|l1 t1|l1|l1 t1];
-case: t2=> [n2|t21 t22|l2|l2 b2|l2 t2|l2|l2 t2] /=;
+elim: t1 t2=> [n1|t11 IH1 t12 IH2|l1|l1 b1|l1 t1 IH1|l1|l1 t1 IH1];
+case=> [n2|t21 t22|l2|l2 b2|l2 t2|l2|l2 t2] /=;
 wp_rec; wp_pures=> //.
 - iPureIntro; congr (# (LitBool _)).
   apply: bool_decide_iff; intuition congruence.
 - wp_bind (eq_term _ _).
-  iApply (wp_wand with "IH"); iIntros (?) "->".
+  iPoseProof (IH1 t21) as "IH1"; iPoseProof (IH2 t22) as "IH2".
+  iApply (twp_wand with "IH1"); iIntros (?) "->".
   case: bool_decide_reflect=> e1.
-  + wp_pures; iApply (wp_wand with "IH"); iIntros (?) "->".
+  + wp_pures; iApply (twp_wand with "IH2"); iIntros (?) "->".
     iPureIntro; congr (# (LitBool _)).
     apply: bool_decide_iff; intuition congruence.
   + wp_pures; iPureIntro; congr (# (LitBool _)).
@@ -57,7 +69,9 @@ wp_rec; wp_pures=> //.
   + wp_pures; iPureIntro; congr (# (LitBool _)).
     rewrite bool_decide_false; congruence.
 - case: bool_decide_reflect=> e1.
-  + wp_pures; iApply (wp_wand with "IH"); iIntros (?) "->".
+  + wp_pures.
+    iPoseProof (IH1 t2) as "IH1".
+    iApply (twp_wand with "IH1"); iIntros (?) "->".
     iPureIntro; congr (# (LitBool _)).
     apply: bool_decide_iff; intuition congruence.
   + wp_pures; iPureIntro; congr (# (LitBool _)).
@@ -65,7 +79,9 @@ wp_rec; wp_pures=> //.
 - iPureIntro; congr (# (LitBool _)).
   apply: bool_decide_iff; intuition congruence.
 - case: bool_decide_reflect=> e1.
-  + wp_pures; iApply (wp_wand with "IH"); iIntros (?) "->".
+  + wp_pures.
+    iPoseProof (IH1 t2) as "IH1".
+    iApply (twp_wand with "IH1"); iIntros (?) "->".
     iPureIntro; congr (# (LitBool _)).
     apply: bool_decide_iff; intuition congruence.
   + wp_pures; iPureIntro; congr (# (LitBool _)).
