crypto.v
@@ -581,7 +581,7 @@ iCombine "Hspec Hj" as "Hspec".
 by iApply "Hswp".
 Qed.
 
-Lemma wp_eq_term2 v11 v12 v21 v22 j K :
+Lemma twp_eq_term2 v11 v12 v21 v22 j K :
   lo_term v11 v12 -∗
   lo_term v21 v22 -∗
   symbols_inv term_names -∗
@@ -589,15 +589,15 @@ Lemma wp_eq_term2 v11 v12 v21 v22 j K :
   spec_ctx -∗
   j ⤇ fill K (eq_term v12 v22) -∗
   WP eq_term v11 v21
-     {{ v, ⌜v = #(bool_decide (v11 = v21))⌝ ∗ j ⤇ fill K v }}.
+     [{ v, ⌜v = #(bool_decide (v11 = v21))⌝ ∗ j ⤇ fill K v }].
 Proof.
 iDestruct 1 as (t11 t12) "(-> & -> & #Ht1)".
 iDestruct 1 as (t21 t22) "(-> & -> & #Ht2)".
-iIntros "Hsymb Hopaque Hspec Hj"; iApply fupd_wp.
+iIntros "Hsymb Hopaque Hspec Hj"; iApply fupd_twp.
 iPoseProof (step_eq_term t12 t22) as "Hswp".
 iMod (swp_elim with "Hswp Hspec Hj") as (v) "[Hj ->]"; first done.
-iModIntro; iPoseProof (wp_eq_term t11 t21) as "Hwp".
-iApply (wp_wand with "Hwp"); iIntros (v) "->".
+iModIntro; iPoseProof (twp_eq_term t11 t21) as "Hwp".
+iApply (twp_wand with "Hwp"); iIntros (v) "->".
 iAssert ⌜bool_decide (t12 = t22) = bool_decide (t11 = t21)⌝%I
         with "[Hsymb Hopaque]" as "->".
   iPoseProof (lo_term_aux_perm with "Hsymb Hopaque Ht1 Ht2") as "%HE".
